src/dafny/utils/Helpers.dfy
@@ -11,4 +11,22 @@ module Helpers {
     /* Either type */
     datatype Either<T> = Left(T) | Right(T)
 
+    /**
+     *  Ceiling function.
+     *
+     *  @param  n   Numerator
+     *  @param  d   Denominator
+     *  @returns    The smallest integer last than float(n / d).
+     */
+    function ceil(n: nat, d: nat) : nat
+        requires d != 0
+        ensures n >= 1 ==> ceil(n , d) >= 1
+        ensures ceil(n ,d) == 0 <==> n == 0
+    {
+        if (n % d == 0) then 
+            n / d
+        else 
+            n / d + 1
+    }       
+
 }
