src/dafny/ssz/BytesAndBits.dfy
@@ -1,0 +1,132 @@
+include "../utils/Eth2Types.dfy"
+
+/**
+ *  Helpers to convert list of bits into uint8 and back
+ *
+ */
+ module BytesAndBits {
+
+    import opened Eth2Types
+
+    /** Convert a boolean into a Byte.
+     *
+     *  @param      b   A boolean.
+     *  @returns        A Byte (uint8) such that b?1:0. 
+     */
+    function method boolToByte(b : bool) : Byte
+        ensures 0 <= boolToByte(b) <= 1  
+    {
+        (if b then 1 else 0) as Byte
+    }
+
+    /**
+     *  Convert a Byte into a boolean.
+     *
+     *  @param      b   A byte between 0 and 1.
+     *  @returns        The corresponding boolean (b == 1)?true:false.
+     */
+    function method byteToBool(b : Byte) : bool
+        requires 0 <= b <= 1
+    {
+        b == 1
+    }
+
+    /**
+     *  Check if a sequence of booleans contains only false.
+     *  
+     *  @param  l   A sequence of bits.
+     *  @returns    true iff all the bits in l are false. 
+     *
+     *  @note       isNull([]) is vacuously true (the forall trivially holds).
+     */
+    predicate isNull(l : seq<bool>) 
+    {
+        forall i | 0 <= i < |l| :: !l[i]
+    }
+
+    /**
+     *  Convert a list of 8 bits into a number.
+     *
+     *  @param  l   A sequence of bits.
+     *  @returns    A byte the binary encoding of which is reverse(l).
+     */
+    function method list8BitsToByte(l : seq<bool>) : Byte    
+        requires |l| == 8 
+        ensures isNull(l) <==> list8BitsToByte(l) == 0
+    {
+        128 * boolToByte(l[7]) +
+        64 * boolToByte(l[6]) +
+        32 * boolToByte(l[5]) +
+        16 * boolToByte(l[4]) +
+        8 * boolToByte(l[3]) +
+        4 * boolToByte(l[2]) +
+        2 * boolToByte(l[1]) +
+        1 * boolToByte(l[0])
+    }
+
+    /**
+     *  Compute a list of bits given a Byte.
+     *
+     *  @param  n   A byte, i.e. a number that can be represented with 8 bits.
+     *  @returns    A sequence of bits `l` such `reverse(l)` is the binary encoding of `n`. 
+     */
+    function method byteTo8Bits( n : Byte ) : seq<bool>
+        ensures | byteTo8Bits(n) | == 8 
+    {
+        [
+            byteToBool((n / 1) % 2),
+            byteToBool((n / 2) % 2),
+            byteToBool((n / 4) % 2), 
+            byteToBool((n / 8) % 2),
+            byteToBool((n / 16) % 2),
+            byteToBool((n / 32) % 2),
+            byteToBool((n / 64) % 2),
+            byteToBool((n / 128) % 2)
+        ]
+    }
+
+    //  Some useful properties.
+
+    /** 
+     *  Encode(decode(n)) = Identity(n).
+     *  
+     *  @param  n   a number.
+     *  @returns    Encoding (as a Byte) the decoded version of `n` yields `n`.
+     */
+    lemma encodeOfDecodeByteIsIdentity(n: Byte)  
+        ensures list8BitsToByte(byteTo8Bits(n)) == n 
+    {   //  Thanks Dafny.
+    }
+
+    /** 
+     *  Decode(encode(l)) = Identity(l).
+     *  
+     *  @param  l   a list of 8 bits.
+     *  @returns    Decoding (as a list of bits) the encoded version of `l` yields `l`.
+     *
+     */    
+     lemma decodeOfEncode8BitsIsIdentity(l : seq<bool>) 
+        requires |l| == 8
+        ensures byteTo8Bits(list8BitsToByte(l)) == l 
+    {   //  Thanks Dafny.
+    }
+
+    /** 
+     *  Zero is the only byte represented by the null sequence.
+     *
+     *  @param  n   A Byte
+     */
+    lemma byteIsZeroIffBinaryIsNull(n : Byte) 
+        ensures n == 0 <==> isNull(byteTo8Bits(n))
+    {
+        calc <==> {
+            n == 0;
+            <==> {  //   This can be omitted as Dafny  uses it anyway. 
+                    encodeOfDecodeByteIsIdentity(n); 
+                 } 
+            list8BitsToByte(byteTo8Bits(n)) == 0;
+            <==>  //    Ensures of list8BitsToByte
+            isNull(byteTo8Bits(n));
+        }
+    }
+ }
